Advance proofs: groups in 2nd part, quantifier in 1st part

warblreequiv/LWEquivTMatcher.v
@@ -1,5 +1,5 @@
 From Coq Require Import PeanoNat ZArith Bool Lia Program.Equality List Program.Wf.
-From Linden Require Import Tree LindenParameters CharsWarblre TMatching.
+From Linden Require Import Tree LindenParameters CharsWarblre TMatching Chars.
 From Warblre Require Import Patterns Result Notation Errors Node RegExpRecord Base Coercions Semantics Typeclasses.
 Import Patterns.
 Import Result.Result.
@@ -90,200 +90,346 @@ Fixpoint tree_res' (t:tree) (s: MatchState) (gl: open_groups): Result (option Ma
   end.
 
 
-Definition equiv_tree (mc: MatcherContinuation) (tmc: TMatcherContinuation) (gl: open_groups) :=
-  forall s: MatchState, 
-  match tmc s, mc s with
-  | Error _, _ | _, Error _ => True (* finer modeling? *)
-  | Success t, Success res => tree_res' t s gl = Success res
-  end.
+Section Main.
+  Context (s0: string).
 
-Definition id_mcont: MatcherContinuation := fun x => Success (Some x).
-Definition id_tmcont: TMatcherContinuation := fun _ => Success Match.
+  Definition equiv_results (s: MatchState) (gl: open_groups) (res': MatchResult) (t': TMatchResult) :=
+    match t', res' with
+    | Error _, _ | _, Error _ => True (* finer modeling? *)
+    | Success t, Success res => tree_res' t s gl = Success res
+    end.
 
-Lemma id_equiv: equiv_tree id_mcont id_tmcont nil.
-Proof.
-  intro s. simpl. reflexivity.
-Qed.
+  Definition equiv_tree_mcont (mc: MatcherContinuation) (tmc: TMatcherContinuation) (gl: open_groups) :=
+    forall s: MatchState,
+    MatchState.input s = s0 -> 
+    equiv_results s gl (mc s) (tmc s).
 
+  Definition equiv_tree_matcher (m: Matcher) (tm: TMatcher) :=
+    forall mc tmc gl, equiv_tree_mcont mc tmc gl -> equiv_tree_mcont (fun s => m s mc) (fun s => tm s tmc) gl.
 
-Theorem compile_tcompile: forall reg ctx rer,
-  let m' := Semantics.compileSubPattern reg ctx rer forward in
-  let tm' := tCompileSubPattern reg ctx rer forward in
-  match m', tm' with
-  | Error _, _ | _, Error _ => True
-  | Success m, Success tm =>
-  forall mc tmc gl, equiv_tree mc tmc gl -> equiv_tree (fun s => m s mc) (fun s => tm s tmc) gl
-  end.
-Proof.
-  intros reg ctx rer.
-  revert ctx.
-  induction reg; simpl.
+  Definition id_mcont: MatcherContinuation := fun x => Success (Some x).
+  Definition id_tmcont: TMatcherContinuation := fun _ => Success Match.
 
-  - (* Empty *)
-    intros. unfold equiv_tree in *. assumption.
-  
-  - (* Character *)
-    intros. unfold equiv_tree in *. intro.
-    unfold tCharacterSetMatcher, Semantics.characterSetMatcher.
-    simpl.
-    remember ((_ <? 0)%Z || _) as b.
-    destruct b.
-    + simpl. reflexivity.
-    + remember (Z.min _ _) as index.
-      remember (List.List.Indexing.Int.indexing _ _) as chr'.
-      destruct chr'; simpl; try (exact I).
-      remember (if CharSet.exist_canonicalized _ _ _ then false else true) as b2.
-      destruct b2; simpl.
-      1: reflexivity.
-      remember (match_state _ _ _) as s'.
-      specialize (H s').
-      destruct (tmc s'); simpl; try exact I.
-      destruct (mc s'); simpl; try exact I.
-      replace (Z.min (MatchState.endIndex s) (MatchState.endIndex s + 1)) with (MatchState.endIndex s) in Heqindex by lia.
-      rewrite Heqindex in Heqchr'.
-      replace (nth _ _ s0) with s0 by admit.
-      rewrite EqDec.reflb.
-      rewrite <- H.
-      f_equal.
-      unfold advance_ms.
-      rewrite Heqs'.
-      reflexivity.
-  
-  - (* Dot; mostly same as character *)
-    intros.
-    intro s.
-    unfold tCharacterSetMatcher, Semantics.characterSetMatcher.
-    simpl.
-    remember ((_ <? 0)%Z || _) as b.
-    destruct b.
-    + simpl. reflexivity.
-    + remember (Z.min _ _) as index.
-      remember (List.List.Indexing.Int.indexing _ _) as chr'.
-      destruct chr'; simpl; try (exact I).
-      remember (if CharSet.exist_canonicalized _ _ _ then false else true) as b2.
-      destruct b2; simpl.
-      1: reflexivity.
-      remember (match_state _ _ _) as s'.
-      specialize (H s').
-      destruct (tmc s'); simpl; try exact I.
-      destruct (mc s'); simpl; try exact I.
-      replace (Z.min (MatchState.endIndex s) (MatchState.endIndex s + 1)) with (MatchState.endIndex s) in Heqindex by lia.
-      rewrite Heqindex in Heqchr'.
-      replace (nth _ _ s0) with s0 by admit.
-      rewrite EqDec.reflb.
-      rewrite <- H.
-      f_equal.
-      unfold advance_ms.
-      rewrite Heqs'.
-      reflexivity.
-  
-  - (* Unsupported case *)
-    intro. destruct (match ae with | DecimalEsc de => _ | ACharacterClassEsc cce => _ | ACharacterEsc ce => _ | GroupEsc gn => _ end); split.
-  
-  - (* Character class: unsupported *)
-    intro. destruct (let! _ =<< _ in _); split.
-  
-  - (* Disjunction *)
-    intro.
-    remember (Disjunction_left reg2 :: ctx) as ctxleft.
-    remember (Disjunction_right reg1 :: ctx) as ctxright.
-    specialize (IHreg1 ctxleft).
-    specialize (IHreg2 ctxright).
-    destruct (Semantics.compileSubPattern reg1 _ _ _) as [m1|] eqn:?; simpl; try exact I.
-    destruct (Semantics.compileSubPattern reg2 _ _ _) as [m2|] eqn:?; simpl; try exact I.
-    destruct (tCompileSubPattern reg1 _ _ _) as [tm1|] eqn:?; simpl; try exact I.
-    destruct (tCompileSubPattern reg2 _ _ _) as [tm2|] eqn:?; simpl; try exact I.
-    simpl in *.
-    intros.
-    intro s'.
-    specialize (IHreg1 mc tmc gl H s').
-    specialize (IHreg2 mc tmc gl H s').
-    simpl in *.
-    destruct (tm1 s' tmc) as [t1|] eqn:?; simpl; try exact I.
-    destruct (tm2 s' tmc) as [t2|] eqn:?; simpl; try exact I.
-    destruct (m1 s' mc) as [r|] eqn:?; simpl; try exact I.
-    destruct r eqn:?; simpl.
-    + rewrite IHreg1. simpl. reflexivity.
-    + destruct (m2 s' mc) as [r2|] eqn:?; simpl; try exact I.
-      rewrite IHreg1. simpl. assumption.
-  
-  - (* Quantifier *)
-    intro.
-    admit.
-  
-  - (* Sequence *)
-    intro.
-    remember (Seq_left reg2 :: ctx) as ctxleft.
-    remember (Seq_right reg1 :: ctx) as ctxright.
-    specialize (IHreg1 ctxleft).
-    specialize (IHreg2 ctxright).
-    destruct (Semantics.compileSubPattern reg1 _ _ _) as [m1|] eqn:?; simpl; try exact I.
-    destruct (Semantics.compileSubPattern reg2 _ _ _) as [m2|] eqn:?; simpl; try exact I.
-    destruct (tCompileSubPattern reg1 _ _ _) as [tm1|] eqn:?; simpl; try exact I.
-    destruct (tCompileSubPattern reg2 _ _ _) as [tm2|] eqn:?; simpl; try exact I.
-    simpl in *.
-    intros. intro.
-    specialize (IHreg2 mc tmc gl H).
-    specialize (IHreg1 (fun s0 => m2 s0 mc) (fun s0 => tm2 s0 tmc) gl IHreg2 s).
-    simpl in *.
-    assumption.
-  
-  - (* Group *)
-    intro.
-    remember (Group_inner name :: ctx) as ctx'.
-    specialize (IHreg ctx').
-    destruct (Semantics.compileSubPattern reg ctx' rer forward) as [m|] eqn:?; simpl; try exact I.
-    destruct (tCompileSubPattern reg ctx' rer forward) as [tm|] eqn:?; simpl; try exact I.
-    intros mc tmc gl H s.
-    simpl in *.
-    remember (fun y : MatchState => _) as treecont.
-    remember (fun y : MatchState => let! r =<< _ in let! cap =<< _ in mc _) as origcont.
-    remember (StaticSemantics.countLeftCapturingParensBefore _ ctx + 1) as gid.
-    set (gl' := (gid, MatchState.endIndex s)::gl).
-    specialize (IHreg origcont treecont gl').
-    assert (equiv_tree origcont treecont gl') as Hequivcont.
-    {
-      intro y.
-      rewrite Heqtreecont, Heqorigcont.
-      remember (MatchState.endIndex s) as x.
-      destruct negb eqn:?; simpl; try exact I.
-      destruct (gid =? 0) eqn:?; simpl; try exact I.
-      destruct List.List.Update.Nat.One.update eqn:?; simpl; try exact I.
-      remember (match_state _ _ s0) as s'.
-      destruct (tmc s') as [t|] eqn:?; simpl; try exact I.
-      destruct (mc s') as [res|] eqn:?; simpl; try exact I.
-      rewrite EqDec.reflb. simpl.
-      rewrite Heqb0.
-      (* Prove: the result of List.List.....Update does not depend on the type of the error that should be returned if any *)
-      replace (@List.List.Update.Nat.One.update _ tree_res'_error _ _ _ (gid - 1)) with (@Success _ tree_res'_error s0) by admit.
+  Lemma id_equiv: equiv_tree_mcont id_mcont id_tmcont nil.
+  Proof.
+    intros s Hss0. simpl. reflexivity.
+  Qed.
+
+  Lemma repeatMatcher'_tRepeatMatcher': forall (m: Matcher) (tm: TMatcher),
+    equiv_tree_matcher m tm ->
+    forall fuel: nat,
+    forall (mc: MatcherContinuation) (tmc: TMatcherContinuation) (gl: open_groups),
+    equiv_tree_mcont mc tmc gl ->
+    forall (min: non_neg_integer) (max: non_neg_integer_or_inf) (greedy: bool)
+    (x: MatchState) (parenIndex parenCount: non_neg_integer),
+    MatchState.input x = s0 ->
+    equiv_results x gl
+      (Semantics.repeatMatcher' m min max greedy x mc parenIndex parenCount fuel)
+      (tRepeatMatcher' tm min max greedy x tmc parenIndex parenCount fuel).
+  Proof.
+    intros m tm Hm_tm_equiv fuel.
+    induction fuel as [|fuel IHfuel].
+    - simpl. split.
+    - intros mc tmc gl Hequivcont min max greedy x parenIndex parenCount Hxs0.
+      unfold equiv_results.
       simpl.
-      specialize (H s').
-      rewrite Heqt, Heqm0 in H.
-      rewrite Heqs' in H.
-      (* mismatching inputs... but all the match states that we manipulate here use the same input, morally *)
-      admit.
-    }
-    specialize (IHreg Hequivcont s).
-    simpl in *.
-    destruct (tm s treecont) as [t|] eqn:?; simpl; try exact I.
-    destruct (m s origcont) as [res|] eqn:?; simpl; try exact I.
-    assumption.
-  
-  
-  - (* Unsupported *)
-    split.
-  - (* Unsupported *)
-    split.
-  - (* Unsupported *)
-    split.
-  - (* Unsupported *)
-    split.
-  - (* Lookahead: unsupported *)
-    intro. destruct (let! _ =<< _ in _); split.
-  - (* Negative lookahead: unsupported *)
-    intro. destruct (let! _ =<< _ in _); split.
-  - (* Lookbehind: unsupported *)
-    intro. destruct (let! _ =<< _ in _); split.
-  - (* Negative lookbehind: unsupported *)
-    intro. destruct (let! _ =<< _ in _); split.
-Admitted.
+      destruct (max =? 0)%NoI eqn:Hmax0; simpl.
+      (* Case max = 0: use hypothesis on continuation *)
+      + unfold equiv_tree_mcont in Hequivcont.
+        apply Hequivcont. assumption.
+      (* Case max > 0 *)
+      + (* Assume that the capture reset succeeds *)
+        destruct List.List.Update.Nat.Batch.update as [cap'|] eqn:Heqcap'; simpl. 2: exact I.
+        rewrite Hxs0.
+        remember (match_state s0 (MatchState.endIndex x) cap') as s'.
+        remember (fun y: MatchState => _) as tmc'.
+        remember (fun (y: MatchState) => (_: MatchResult)) as mc'.
+        assert (equiv_tree_mcont mc' tmc' gl) as Hequiv'.
+        {
+          intros s Hss0.
+          rewrite Heqmc', Heqtmc'.
+          unfold equiv_results.
+          destruct ((min ==? 0)%wt && _) eqn:Hprogress; simpl.
+          - reflexivity.
+          - remember (if (min ==? 0)%wt then 0 else min - 1) as min'.
+            remember (if (max =? +∞)%NoI then +∞ else (max - 1)%NoI) as max'.
+            specialize (IHfuel mc tmc gl Hequivcont min' max' greedy s parenIndex parenCount Hss0).
+            unfold equiv_results in IHfuel.
+            destruct tRepeatMatcher' as [subtree|] eqn:Heqsubtree; simpl. 2: exact I.
+            destruct Semantics.repeatMatcher' as [res|] eqn:Heqres; simpl. 2: exact I.
+            apply IHfuel.
+        }
+        assert (equiv_results s' gl (m s' mc') (tm s' tmc')) as Hequivres.
+        {
+          unfold equiv_tree_matcher in Hm_tm_equiv.
+          specialize (Hm_tm_equiv mc' tmc' gl Hequiv' s').
+          assert (Hs's0: MatchState.input s' = s0).
+          {
+            rewrite Heqs'. reflexivity.
+          }
+          specialize (Hm_tm_equiv Hs's0).
+          unfold equiv_results in Hm_tm_equiv.
+          unfold equiv_results.
+          destruct tm as [subtree|] eqn:Heqsubtree; simpl. 2: exact I.
+          destruct m as [res|] eqn:Heqres; simpl. 2: exact I.
+          apply Hm_tm_equiv.
+        }
+        assert ((reset_groups_ms (seq (parenIndex + 1) parenCount) x) = (@Success MatchState tree_res'_error s')) as RESET_GROUPS by admit.
+        destruct (negb (min =? 0)) eqn:Hmin_nonzero; simpl.
+        (* Case min > 0 *)
+        * unfold equiv_results in Hequivres.
+          destruct tm as [subtree|] eqn:Heqsubtree; simpl. 2: exact I.
+          destruct m as [res|] eqn:Heqres; simpl. 2: exact I.
+          (* Resetting the groups from parenIndex + 1 to parenIndex + parenCount in x yields exactly state s',
+            see Heqs' and Heqcap'. Let's admit that for now *)
+          rewrite RESET_GROUPS.
+          simpl.
+          apply Hequivres.
+        (* Case min = 0 *)
+        * specialize (Hequivcont x Hxs0).
+          unfold equiv_results in Hequivcont, Hequivres.
+          destruct greedy eqn:Hgreedy; simpl.
+          -- destruct tm as [z|] eqn:Heqz; simpl. 2: exact I.
+             destruct tmc as [z'|] eqn:Heqz'; simpl. 2: exact I.
+             rewrite RESET_GROUPS.
+             destruct m as [zm|] eqn:Heqzm; simpl. 2: exact I.
+             unfold "!=?".
+             destruct (zm ==? None)%wt eqn:Hzm_None; simpl.
+             ++ rewrite Hequivres. simpl.
+                rewrite EqDec.inversion_true in Hzm_None.
+                rewrite Hzm_None.
+                destruct mc.
+                2: exact I.
+                assumption.
+             ++ rewrite Hequivres. simpl.
+                rewrite EqDec.inversion_false in Hzm_None.
+                destruct zm; simpl.
+                ** reflexivity.
+                ** contradiction.
+          -- destruct tmc as [z'|] eqn:Heqz'; simpl. 2: exact I.
+             destruct tm as [z|] eqn:Heqz; simpl. 2: exact I.
+             rewrite RESET_GROUPS.
+             destruct mc as [zmc|] eqn:Heqzmc; simpl. 2: exact I.
+             unfold "!=?".
+             destruct (zmc ==? None)%wt eqn:Hzmc_None; simpl.
+             ++ destruct m; simpl. 2: exact I.
+                rewrite Hequivcont. simpl.
+                rewrite EqDec.inversion_true in Hzmc_None.
+                rewrite Hzmc_None.
+                assumption.
+             ++ rewrite Hequivcont. simpl.
+                rewrite EqDec.inversion_false in Hzmc_None.
+                destruct zmc; simpl.
+                ** reflexivity.
+                ** contradiction.
+  Admitted.
+
+
+  Theorem compile_tcompile: forall reg ctx rer,
+    let m' := Semantics.compileSubPattern reg ctx rer forward in
+    let tm' := tCompileSubPattern reg ctx rer forward in
+    match m', tm' with
+    | Error _, _ | _, Error _ => True
+    | Success m, Success tm => equiv_tree_matcher m tm
+    end.
+  Proof.
+    intros reg ctx rer.
+    revert ctx.
+    induction reg; simpl.
+
+    - (* Empty *)
+      unfold equiv_tree_matcher. intros. unfold equiv_tree_mcont in *. assumption.
+    
+    - (* Character *)
+      intros _ mc tmc gl Hequiv. unfold equiv_tree_mcont in *. intros s Hss0.
+      unfold tCharacterSetMatcher, Semantics.characterSetMatcher.
+      simpl.
+      remember ((_ <? 0)%Z || _) as b.
+      destruct b.
+      + simpl. reflexivity.
+      + remember (Z.min _ _) as index.
+        remember (List.List.Indexing.Int.indexing _ _) as chr'.
+        destruct chr' as [chr'|]; simpl; try (exact I).
+        remember (if CharSet.exist_canonicalized _ _ _ then false else true) as b2.
+        destruct b2; simpl.
+        1: reflexivity.
+        remember (match_state _ _ _) as s'.
+        specialize (Hequiv s').
+        assert (MatchState.input s' = s0) as Hs's0.
+        {
+          rewrite Heqs'. simpl. apply Hss0.
+        }
+        specialize (Hequiv Hs's0).
+        destruct (tmc s') as [child|]; simpl; try exact I.
+        destruct (mc s') as [res|]; simpl; try exact I.
+        replace (Z.min (MatchState.endIndex s) (MatchState.endIndex s + 1)) with (MatchState.endIndex s) in Heqindex by lia.
+        rewrite Heqindex in Heqchr'.
+        replace (nth _ _ chr') with chr' by admit.
+        rewrite EqDec.reflb.
+        rewrite <- Hequiv.
+        f_equal.
+        unfold advance_ms.
+        rewrite Heqs'.
+        reflexivity.
+    
+    - (* Dot; same as character *)
+      intros _ mc tmc gl Hequiv. unfold equiv_tree_mcont in *. intros s Hss0.
+      unfold tCharacterSetMatcher, Semantics.characterSetMatcher.
+      simpl.
+      remember ((_ <? 0)%Z || _) as b.
+      destruct b.
+      + simpl. reflexivity.
+      + remember (Z.min _ _) as index.
+        remember (List.List.Indexing.Int.indexing _ _) as chr'.
+        destruct chr' as [chr'|]; simpl; try (exact I).
+        remember (if CharSet.exist_canonicalized _ _ _ then false else true) as b2.
+        destruct b2; simpl.
+        1: reflexivity.
+        remember (match_state _ _ _) as s'.
+        specialize (Hequiv s').
+        assert (MatchState.input s' = s0) as Hs's0.
+        {
+          rewrite Heqs'. simpl. apply Hss0.
+        }
+        specialize (Hequiv Hs's0).
+        destruct (tmc s') as [child|]; simpl; try exact I.
+        destruct (mc s') as [res|]; simpl; try exact I.
+        replace (Z.min (MatchState.endIndex s) (MatchState.endIndex s + 1)) with (MatchState.endIndex s) in Heqindex by lia.
+        rewrite Heqindex in Heqchr'.
+        replace (nth _ _ chr') with chr' by admit.
+        rewrite EqDec.reflb.
+        rewrite <- Hequiv.
+        f_equal.
+        unfold advance_ms.
+        rewrite Heqs'.
+        reflexivity.
+    
+    - (* Atom escape: unsupported *)
+      intro. destruct (match ae with | DecimalEsc de => _ | ACharacterClassEsc cce => _ | ACharacterEsc ce => _ | GroupEsc gn => _ end); split.
+    
+    - (* Character class: unsupported *)
+      intro. destruct (let! _ =<< _ in _); split.
+    
+    - (* Disjunction *)
+      intro ctx.
+      remember (Disjunction_left reg2 :: ctx) as ctxleft.
+      remember (Disjunction_right reg1 :: ctx) as ctxright.
+      specialize (IHreg1 ctxleft).
+      specialize (IHreg2 ctxright).
+      destruct (Semantics.compileSubPattern reg1 _ _ _) as [m1|] eqn:?; simpl; try exact I.
+      destruct (Semantics.compileSubPattern reg2 _ _ _) as [m2|] eqn:?; simpl; try exact I.
+      destruct (tCompileSubPattern reg1 _ _ _) as [tm1|] eqn:?; simpl; try exact I.
+      destruct (tCompileSubPattern reg2 _ _ _) as [tm2|] eqn:?; simpl; try exact I.
+      simpl in *.
+      intros mc tmc gl Hequiv s' Hs's0.
+      specialize (IHreg1 mc tmc gl Hequiv s' Hs's0).
+      specialize (IHreg2 mc tmc gl Hequiv s' Hs's0).
+      simpl in *.
+      destruct (tm1 s' tmc) as [t1|] eqn:?; simpl; try exact I.
+      destruct (tm2 s' tmc) as [t2|] eqn:?; simpl; try exact I.
+      destruct (m1 s' mc) as [r|] eqn:?; simpl; try exact I.
+      destruct r eqn:?; simpl.
+      + rewrite IHreg1. simpl. reflexivity.
+      + destruct (m2 s' mc) as [r2|] eqn:?; simpl; try exact I.
+        rewrite IHreg1. simpl. assumption.
+    
+    - (* Quantifier *)
+      intro ctx.
+      remember (Quantified_inner q :: ctx) as ctx'.
+      specialize (IHreg ctx').
+      destruct Semantics.compileSubPattern as [m|] eqn:Heqm; simpl. 2: exact I.
+      destruct tCompileSubPattern as [tm|] eqn:Heqtm; simpl. 2: destruct (if (negb _) then _ else _); exact I.
+      simpl in IHreg.
+      destruct negb; simpl. 1: exact I.
+      unfold equiv_tree_matcher.
+      intros mc tmc gl Hequivcont. unfold equiv_tree_mcont.
+      intros s Hss0.
+      unfold Semantics.repeatMatcher.
+      unfold tRepeatMatcher.
+      now apply repeatMatcher'_tRepeatMatcher'.
+    
+    - (* Sequence *)
+      intro ctx.
+      remember (Seq_left reg2 :: ctx) as ctxleft.
+      remember (Seq_right reg1 :: ctx) as ctxright.
+      specialize (IHreg1 ctxleft).
+      specialize (IHreg2 ctxright).
+      destruct (Semantics.compileSubPattern reg1 _ _ _) as [m1|] eqn:?; simpl; try exact I.
+      destruct (Semantics.compileSubPattern reg2 _ _ _) as [m2|] eqn:?; simpl; try exact I.
+      destruct (tCompileSubPattern reg1 _ _ _) as [tm1|] eqn:?; simpl; try exact I.
+      destruct (tCompileSubPattern reg2 _ _ _) as [tm2|] eqn:?; simpl; try exact I.
+      simpl in *.
+      intros mc tmc gl Hequiv s Hss0.
+      specialize (IHreg2 mc tmc gl Hequiv).
+      specialize (IHreg1 (fun s0 => m2 s0 mc) (fun s0 => tm2 s0 tmc) gl IHreg2 s Hss0).
+      simpl in *.
+      assumption.
+    
+    - (* Group *)
+      intro ctx.
+      remember (Group_inner name :: ctx) as ctx'.
+      specialize (IHreg ctx').
+      destruct (Semantics.compileSubPattern reg ctx' rer forward) as [m|] eqn:Heqm; simpl; try exact I.
+      destruct (tCompileSubPattern reg ctx' rer forward) as [tm|] eqn:Heqtm; simpl; try exact I.
+      intros mc tmc gl Hequiv s Hss0.
+      simpl in *.
+      unfold equiv_results.
+      remember (fun y : MatchState => _) as treecont.
+      remember (fun y : MatchState => let! r =<< _ in let! cap =<< _ in mc _) as origcont.
+      remember (StaticSemantics.countLeftCapturingParensBefore _ ctx + 1) as gid.
+      set (gl' := (gid, MatchState.endIndex s)::gl).
+      specialize (IHreg origcont treecont gl').
+      assert (equiv_tree_mcont origcont treecont gl') as Hequivcont.
+      {
+        intros y Hys0.
+        rewrite Heqtreecont, Heqorigcont.
+        remember (MatchState.endIndex s) as i.
+        destruct negb eqn:Hi_le_y; simpl; try exact I.
+        destruct (gid =? 0) eqn:Hgid_nonzero; simpl; try exact I.
+        destruct List.List.Update.Nat.One.update as [cap'|] eqn:Hcapupd; simpl; try exact I.
+        remember (match_state _ _ cap') as s'.
+        destruct (tmc s') as [t|] eqn:Heqt; simpl; try exact I.
+        destruct (mc s') as [res|] eqn:Heqres; simpl; try exact I.
+        rewrite EqDec.reflb. simpl.
+        rewrite Hgid_nonzero.
+        (* Prove: the result of List.List.....Update does not depend on the type of the error that should be returned if any *)
+        replace (@List.List.Update.Nat.One.update _ tree_res'_error _ _ _ (gid - 1)) with (@Success _ tree_res'_error cap') by admit.
+        simpl.
+        specialize (Hequiv s').
+        assert (MatchState.input s' = s0) as Hs's0.
+        {
+          rewrite Heqs'. simpl. apply Hss0.
+        }
+        specialize (Hequiv Hs's0).
+        rewrite Heqt, Heqres in Hequiv.
+        rewrite Heqs' in Hequiv.
+        rewrite Hss0 in Hequiv.
+        rewrite Hys0.
+        assumption.
+      }
+      specialize (IHreg Hequivcont s Hss0).
+      simpl in *.
+      destruct (tm s treecont) as [t|] eqn:Heqt; simpl; try exact I.
+      destruct (m s origcont) as [res|] eqn:Heqres; simpl; try exact I.
+      assumption.
+    
+    
+    - (* Unsupported *)
+      split.
+    - (* Unsupported *)
+      split.
+    - (* Unsupported *)
+      split.
+    - (* Unsupported *)
+      split.
+    - (* Lookahead: unsupported *)
+      intro. destruct (let! _ =<< _ in _); split.
+    - (* Negative lookahead: unsupported *)
+      intro. destruct (let! _ =<< _ in _); split.
+    - (* Lookbehind: unsupported *)
+      intro. destruct (let! _ =<< _ in _); split.
+    - (* Negative lookbehind: unsupported *)
+      intro. destruct (let! _ =<< _ in _); split.
+  Admitted.
+
+End Main.
